crates/logic/hol/src/syntax/kind/mod.rs
@@ -1,7 +1,0 @@
-//! Kind constructors.
-
-mod arr;
-mod star;
-
-pub use arr::KindArr;
-pub use star::KindStar;
